Replace flor log with ceiling log.

theories/Utils/Arith.v
@@ -34,3 +34,64 @@ Definition lt_sub:
         exists x.
         lia.
   Defined.
+
+(* Ceiling log base 2 function *)
+Definition clog2 (x : nat) : nat := 
+  match x with
+  | 0 => 0
+  | S 0 => 0
+  | S (S n) => S (log2 (S n))
+  end.
+
+Theorem clog2_log2 : forall x,
+  x > 1 -> clog2 (S x) = S (log2 x).
+Proof.
+  intro x; destruct x. { lia. }
+  destruct x. { lia. }
+  reflexivity.
+Qed.
+
+Theorem clog2_ajoint_lem : forall {x}, ~ (2 ^ x < 1).
+Proof.
+  intro x; induction x as [|x IHx].
+  - simpl. lia.
+  - intro. apply IHx. 
+    transitivity (2 ^ S x). 2: { assumption. }
+    simpl. lia.
+Qed.
+
+(* Adjoint theorem/Galois connection defining ceiling log2 *)
+Theorem clog2_lt_pow2 : forall (x y : nat),
+  (2 ^ x < y) <-> (x < clog2 y).
+  intros x y.
+Proof.
+  split; intro.
+  - destruct (1 <? y) eqn:g1y.
+    + rewrite ltb_lt in g1y.
+      destruct y. { lia. } destruct y. { lia. }
+      simpl.
+      rewrite lt_succ_r.
+      rewrite <- log2_le_pow2; lia.
+    + rewrite ltb_nlt in g1y.
+      assert (y = 1) as y1. { lia. }
+      rewrite y1 in H.
+      destruct (clog2_ajoint_lem H).
+  - destruct (1 <? y) eqn:g1y.
+    + rewrite ltb_lt in g1y.
+      destruct y. { lia. }
+      rewrite lt_succ_r.
+      rewrite log2_le_pow2. 2: { lia. }
+      rewrite <- lt_succ_r.
+      destruct y. { lia. }
+      exact H.
+    + rewrite ltb_nlt in g1y.
+      assert (y <= 1). { lia. }
+      destruct (y =? 0) eqn:g0y.
+      * rewrite eqb_eq in g0y.
+        rewrite g0y in H.
+        simpl in H; lia.
+      * rewrite eqb_neq in g0y.
+        assert (y = 1) as y1. { lia. }
+        rewrite y1 in H.
+        simpl in H; lia.
+Qed.
